Extend language with mutually fixpoint.
And separate sum types from product types (no product in Variant/Exn/Eff), and
add Tuple. Also, simplify the AST to use less indirection. This is a huge change.

shift-reset/core/syntax.v
@@ -5,11 +5,20 @@ Inductive binder : Type :=
 | BAny : binder
 | BVar : var -> binder.
 
-Inductive pattern : Type :=
-| PAny : pattern
-| PVar : var -> pattern
-| PConstr : tag -> list binder -> pattern
-| PAlias : pattern -> var -> pattern.
+Inductive variant_pattern : Type :=
+| PVariantAny : variant_pattern
+| PVariantVar : var -> variant_pattern
+| PVariantTag : tag -> binder -> variant_pattern.
+
+Inductive tuple_pattern : Type :=
+| PTupleNil : tuple_pattern
+| PTupleCons : binder -> tuple_pattern -> tuple_pattern.
+
+Inductive record_pattern : Type :=
+| PRecordAny : record_pattern
+| PRecordVar : var -> record_pattern
+| PRecordNil : record_pattern
+| PRecordCons : tag -> binder -> record_pattern -> record_pattern.
 
 Inductive op1 : Type :=
 | Op1Pos : op1
@@ -33,119 +42,131 @@ Inductive term : Type :=
 | TVal : val_term -> term
 | TApp : val_term -> val_term -> term
 | TSeq : term -> term -> term
-| TLet : term -> term1 -> term
+| TLet : binder -> term -> term -> term
 | TIf : val_term -> term -> term -> term
-| TUnpair : val_term -> term2 -> term
-| TCase : val_term -> term1 -> term1 -> term
+| TSplit : binder -> binder -> val_term -> term -> term
+| TCase : val_term -> binder -> term -> binder -> term -> term
 | TWhile : val_term -> term -> term
-| TShift : tag -> term1 -> term
-| TReset : tag -> term -> term
-| TControl : tag -> term1 -> term
-| TPrompt : tag -> term -> term
+| TLetFix : var -> binder -> term -> term -> term
+| TLetFixMut : fix_mut_term -> term -> term
+| TLetTuple : tuple_pattern -> val_term -> term -> term
+| TLetRecord : record_pattern -> val_term -> term -> term
+| TMatchVariant : val_term -> variant_term -> term
+| TShift : binder -> term -> term
+| TReset : term -> term
+| TControl : binder -> term -> term
+| TPrompt : term -> term
 | TRaise : val_term -> term
 | TTry : term -> exn_term -> term
 | TPerform : val_term -> term
 | THandle : term -> ret_term -> eff_term -> term
 | TShallowHandle : term -> ret_term -> eff_term -> term
-| TMatch : val_term -> variant_term -> term
-with term1 : Type :=
-| T1 : binder -> term -> term1
-with term2 : Type :=
-| T2 : binder -> binder -> term -> term2
 with val_term : Type :=
 | TVVar : var -> val_term
-| TVUnit : val_term
+| TVTt : val_term
 | TVInt : Z -> val_term
 | TVFloat : Qc -> val_term
 | TVTrue : val_term
 | TVFalse : val_term
 | TVAnd : val_term -> val_term -> val_term
 | TVOr : val_term -> val_term -> val_term
-| TVFun : term1 -> val_term
-| TVFix : term2 -> val_term
+| TVFun : binder -> term -> val_term
+| TVFix : var -> binder -> term -> val_term
+| TVFixMut : fix_mut_term -> var -> val_term
 | TVPair : val_term -> val_term -> val_term
+| TVTuple : tuple_term -> val_term
+| TVRecord : record_term -> val_term
+| TVProj : val_term -> tag -> val_term
 | TVInl : val_term -> val_term
 | TVInr : val_term -> val_term
+| TVVariant : tag -> val_term -> val_term
 | TVRef : val_term -> val_term
 | TVGet : val_term -> val_term
 | TVSet : val_term -> val_term -> val_term
 | TVFree : val_term -> val_term
-| TVExn : tag -> list val_term -> val_term
-| TVEff : tag -> list val_term -> val_term
+| TVExn : tag -> val_term -> val_term
+| TVEff : tag -> val_term -> val_term
 | TVAssert : val_term -> val_term
 | TVOp1 : op1 -> val_term -> val_term
 | TVOp2 : op2 -> val_term -> val_term -> val_term
-| TVVariant : tag -> list val_term -> val_term
-| TVRecord : record_term -> val_term
-| TVProj : val_term -> tag -> val_term
 with ret_term : Type :=
 | TRetNone : ret_term
 | TRetSome : binder -> term -> ret_term
 with exn_term : Type :=
-| TExnLast : pattern -> term -> exn_term
-| TExnCons : pattern -> term -> exn_term -> exn_term
+| TExnLast : variant_pattern -> term -> exn_term
+| TExnCons : variant_pattern -> term -> exn_term -> exn_term
 with eff_term : Type :=
-| TEffLast : pattern -> binder -> term -> eff_term
-| TEffCons : pattern -> binder -> term -> eff_term -> eff_term
+| TEffLast : variant_pattern -> binder -> term -> eff_term
+| TEffCons : variant_pattern -> binder -> term -> eff_term -> eff_term
 with variant_term : Type :=
 | TVariantNil : variant_term
-| TVariantCons : pattern -> term -> variant_term -> variant_term
+| TVariantCons : variant_pattern -> term -> variant_term -> variant_term
+with tuple_term : Type :=
+| TTupleNil : tuple_term
+| TTupleCons : val_term -> tuple_term -> tuple_term
 with record_term : Type :=
 | TRecordNil : record_term
-| TRecordCons : tag -> val_term -> record_term -> record_term.
+| TRecordCons : tag -> val_term -> record_term -> record_term
+with fix_mut_term : Type :=
+| TFixMutLast : var -> binder -> term -> fix_mut_term
+| TFixMutCons : var -> binder -> term -> fix_mut_term -> fix_mut_term.
 
 Inductive val : Type :=
-| VUnit : val
+| VTt : val
 | VInt : Z -> val
 | VFloat : Qc -> val
 | VTrue : val
 | VFalse : val
-| VFun : fun_clo -> val
-| VFix : fix_clo -> val
+| VFun : binder -> term -> env -> val
+| VFix : var -> binder -> term -> env -> val
+| VFixMut : fix_mut_term -> var -> env -> val
 | VPair : val -> val -> val
+| VTuple : tuple -> val
+| VRecord : record -> val
 | VInl : val -> val
 | VInr : val -> val
+| VVariant : tag -> val -> val
 | VRef : loc -> val
-| VExn : exn -> val
-| VEff : eff -> val
+| VExn : tag -> val -> val
+| VEff : tag -> val -> val
 | VMKPure : metakont -> val
-| VMKReset : metakont -> tag -> val
-| VMKHandle : metakont -> handle_clo -> val
-| VVariant : variant -> val
-| VRecord : record -> val
-with fun_clo : Type :=
-| CFun : env -> term1 -> fun_clo
-with fix_clo : Type :=
-| CFix : env -> term2 -> fix_clo
-with kont_clo : Type :=
-| CKSeq : env -> term -> kont_clo
-| CKLet : env -> term1 -> kont_clo
-with try_clo : Type :=
-| CTry : env -> exn_term -> try_clo
-with handle_clo : Type :=
-| CHandle : env -> ret_term -> eff_term -> handle_clo
-with shallow_handle_clo : Type :=
-| CShallowHandle : env -> ret_term -> eff_term -> shallow_handle_clo
+| VMKReset : metakont -> val
+| VMKHandle : metakont -> ret_term -> eff_term -> env -> val
 with kont : Type :=
 | KNil : kont
-| KCons : kont_clo -> kont -> kont
+| KSeq : term -> env -> kont -> kont
+| KLet : binder -> term -> env -> kont -> kont
 | KApp : kont -> kont -> kont
 with metakont : Type :=
 | MKPure : kont -> metakont
-| MKReset : metakont -> tag -> kont -> metakont
-| MKPrompt : metakont -> tag -> kont -> metakont
-| MKTry : metakont -> try_clo -> kont -> metakont
-| MKHandle : metakont -> handle_clo -> kont -> metakont
-| MKShallowHandle : metakont -> shallow_handle_clo -> kont -> metakont
+| MKReset : metakont -> kont -> metakont
+| MKPrompt : metakont -> kont -> metakont
+| MKTry : metakont -> exn_term -> env -> kont -> metakont
+| MKHandle : metakont -> ret_term -> eff_term -> env -> kont -> metakont
+| MKShallowHandle : metakont -> ret_term -> eff_term -> env -> kont -> metakont
 with env : Type :=
-| EnvNil : env
-| EnvCons : var -> val -> env -> env
-with exn : Type :=
-| Exn : tag -> list val -> exn
-with eff : Type :=
-| Eff : tag -> list val -> eff
-with variant : Type :=
-| Variant : tag -> list val -> variant
+| ENil : env
+| ECons : var -> val -> env -> env
+with tuple : Type :=
+| TupleNil : tuple
+| TupleCons : val -> tuple -> tuple
 with record : Type :=
 | RecordNil : record
 | RecordCons : tag -> val -> record -> record.
+
+Inductive closure : Type :=
+| CFun : binder -> term -> env -> closure
+| CFix : var -> binder -> term -> env -> closure
+| CFixMut : fix_mut_term -> var -> env -> closure
+| CMKPure : metakont -> closure
+| CMKReset : metakont -> closure
+| CMKHandle : metakont -> ret_term -> eff_term -> env -> closure.
+
+Inductive variant : Type :=
+| Variant : tag -> val -> variant.
+
+Inductive exn : Type :=
+| Exn : tag -> val -> exn.
+
+Inductive eff : Type :=
+| Eff : tag -> val -> eff.
