shift-reset/core/coerce.v
@@ -4,7 +4,8 @@ From shift_reset.core Require Import syntax tag var.
 Coercion Tag : string >-> tag.
 Coercion Var : string >-> var.
 Coercion BVar : var >-> binder.
-Coercion PVar : var >-> pattern.
+Coercion PVariantVar : var >-> variant_pattern.
+Coercion PRecordVar : var >-> record_pattern.
 Coercion TVVar : var >-> val_term.
 Coercion TVInt : Z >-> val_term.
 Coercion TVFloat : Qc >-> val_term.
