shift-reset/core/env.v
@@ -1,7 +1,7 @@
 From shift_reset.core Require Import syntax var.
 
-Fixpoint env_lookup (x : var) (env : env) : option val :=
-  match env with
-  | EnvNil => None
-  | EnvCons x' v env' => if var_eqb x x' then Some v else env_lookup x env'
+Fixpoint env_lookup (x : var) (e : env) : option val :=
+  match e with
+  | ENil => None
+  | ECons x' v e' => if var_eqb x x' then Some v else env_lookup x e'
   end.
