shift-reset/core/eq_dec.v
@@ -1,11 +1,10 @@
-From Stdlib Require Import List Qcanon ZArith.
+From Stdlib Require Import Qcanon ZArith.
 From shift_reset.core Require Import syntax loc tag var.
 
 Create HintDb eq_dec_db discriminated.
 
 Hint Resolve Z.eq_dec : eq_dec_db.
 Hint Resolve Qc_eq_dec : eq_dec_db.
-Hint Resolve list_eq_dec : eq_dec_db.
 Hint Resolve loc_eq_dec : eq_dec_db.
 Hint Resolve tag_eq_dec : eq_dec_db.
 Hint Resolve var_eq_dec : eq_dec_db.
@@ -15,10 +14,18 @@ Proof. decide equality; auto with eq_dec_db. Defined.
 
 Hint Resolve binder_eq_dec : eq_dec_db.
 
-Lemma pattern_eq_dec : forall (p1 p2 : pattern), {p1 = p2} + {p1 <> p2}.
+Lemma variant_pattern_eq_dec : forall (p1 p2 : variant_pattern), {p1 = p2} + {p1 <> p2}.
 Proof. decide equality; auto with eq_dec_db. Defined.
 
-Hint Resolve pattern_eq_dec : eq_dec_db.
+Lemma tuple_pattern_eq_dec : forall (p1 p2 : tuple_pattern), {p1 = p2} + {p1 <> p2}.
+Proof. decide equality; auto with eq_dec_db. Defined.
+
+Lemma record_pattern_eq_dec : forall (p1 p2 : record_pattern), {p1 = p2} + {p1 <> p2}.
+Proof. decide equality; auto with eq_dec_db. Defined.
+
+Hint Resolve variant_pattern_eq_dec : eq_dec_db.
+Hint Resolve tuple_pattern_eq_dec : eq_dec_db.
+Hint Resolve record_pattern_eq_dec : eq_dec_db.
 
 Lemma op1_eq_dec : forall (op1 op2 : op1), {op1 = op2} + {op1 <> op2}.
 Proof. decide equality; auto with eq_dec_db. Defined.
@@ -30,53 +37,54 @@ Hint Resolve op1_eq_dec : eq_dec_db.
 Hint Resolve op2_eq_dec : eq_dec_db.
 
 Lemma term_eq_dec : forall (t1 t2 : term), {t1 = t2} + {t1 <> t2}
-with term1_eq_dec : forall (t1 t2 : term1), {t1 = t2} + {t1 <> t2}
-with term2_eq_dec : forall (t1 t2 : term2), {t1 = t2} + {t1 <> t2}
 with val_term_eq_dec : forall (t1 t2 : val_term), {t1 = t2} + {t1 <> t2}
 with ret_term_eq_dec : forall (t1 t2 : ret_term), {t1 = t2} + {t1 <> t2}
 with exn_term_eq_dec : forall (t1 t2 : exn_term), {t1 = t2} + {t1 <> t2}
 with eff_term_eq_dec : forall (t1 t2 : eff_term), {t1 = t2} + {t1 <> t2}
 with variant_term_eq_dec : forall (t1 t2 : variant_term), {t1 = t2} + {t1 <> t2}
-with record_term_eq_dec : forall (t1 t2 : record_term), {t1 = t2} + {t1 <> t2}.
+with tuple_term_eq_dec : forall (t1 t2 : tuple_term), {t1 = t2} + {t1 <> t2}
+with record_term_eq_dec : forall (t1 t2 : record_term), {t1 = t2} + {t1 <> t2}
+with fix_mut_term_eq_dec : forall (t1 t2 : fix_mut_term), {t1 = t2} + {t1 <> t2}.
 Proof. all: decide equality; auto with eq_dec_db. Defined.
 
 Hint Resolve term_eq_dec : eq_dec_db.
-Hint Resolve term1_eq_dec : eq_dec_db.
-Hint Resolve term2_eq_dec : eq_dec_db.
 Hint Resolve val_term_eq_dec : eq_dec_db.
 Hint Resolve ret_term_eq_dec : eq_dec_db.
 Hint Resolve exn_term_eq_dec : eq_dec_db.
 Hint Resolve eff_term_eq_dec : eq_dec_db.
 Hint Resolve variant_term_eq_dec : eq_dec_db.
+Hint Resolve tuple_term_eq_dec : eq_dec_db.
 Hint Resolve record_term_eq_dec : eq_dec_db.
+Hint Resolve fix_mut_term_eq_dec : eq_dec_db.
 
 Lemma val_eq_dec : forall (v1 v2 : val), {v1 = v2} + {v1 <> v2}
-with fun_clo_eq_dec : forall (c1 c2 : fun_clo), {c1 = c2} + {c1 <> c2}
-with fix_clo_eq_dec : forall (c1 c2 : fix_clo), {c1 = c2} + {c1 <> c2}
-with kont_clo_eq_dec : forall (c1 c2 : kont_clo), {c1 = c2} + {c1 <> c2}
-with try_clo_eq_dec : forall (c1 c2 : try_clo), {c1 = c2} + {c1 <> c2}
-with handle_clo_eq_dec : forall (c1 c2 : handle_clo), {c1 = c2} + {c1 <> c2}
-with shallow_handle_clo_eq_dec : forall (c1 c2 : shallow_handle_clo), {c1 = c2} + {c1 <> c2}
 with kont_eq_dec : forall (k1 k2 : kont), {k1 = k2} + {k1 <> k2}
 with metakont_eq_dec : forall (mk1 mk2 : metakont), {mk1 = mk2} + {mk1 <> mk2}
-with env_eq_dec : forall (env1 env2 : env), {env1 = env2} + {env1 <> env2}
-with exn_eq_dec : forall (exn1 exn2 : exn), {exn1 = exn2} + {exn1 <> exn2}
-with eff_eq_dec : forall (eff1 eff2 : eff), {eff1 = eff2} + {eff1 <> eff2}
-with variant_eq_dec : forall (v1 v2 : variant), {v1 = v2} + {v1 <> v2}
+with env_eq_dec : forall (e1 e2 : env), {e1 = e2} + {e1 <> e2}
+with tuple_eq_dec : forall (t1 t2 : tuple), {t1 = t2} + {t1 <> t2}
 with record_eq_dec : forall (r1 r2 : record), {r1 = r2} + {r1 <> r2}.
 Proof. all: decide equality; auto with eq_dec_db. Defined.
 
 Hint Resolve val_eq_dec : eq_dec_db.
-Hint Resolve fun_clo_eq_dec : eq_dec_db.
-Hint Resolve fix_clo_eq_dec : eq_dec_db.
-Hint Resolve kont_clo_eq_dec : eq_dec_db.
-Hint Resolve try_clo_eq_dec : eq_dec_db.
-Hint Resolve handle_clo_eq_dec : eq_dec_db.
-Hint Resolve shallow_handle_clo_eq_dec : eq_dec_db.
 Hint Resolve kont_eq_dec : eq_dec_db.
 Hint Resolve metakont_eq_dec : eq_dec_db.
 Hint Resolve env_eq_dec : eq_dec_db.
+Hint Resolve tuple_eq_dec : eq_dec_db.
+Hint Resolve record_eq_dec : eq_dec_db.
+
+Lemma closure_eq_dec : forall (c1 c2 : closure), {c1 = c2} + {c1 <> c2}.
+Proof. decide equality; auto with eq_dec_db. Defined.
+
+Lemma variant_eq_dec : forall (v1 v2 : variant), {v1 = v2} + {v1 <> v2}.
+Proof. decide equality; auto with eq_dec_db. Defined.
+
+Lemma exn_eq_dec : forall (e1 e2 : exn), {e1 = e2} + {e1 <> e2}.
+Proof. decide equality; auto with eq_dec_db. Defined.
+
+Lemma eff_eq_dec : forall (e1 e2 : eff), {e1 = e2} + {e1 <> e2}.
+Proof. decide equality; auto with eq_dec_db. Defined.
+
+Hint Resolve closure_eq_dec : eq_dec_db.
+Hint Resolve variant_eq_dec : eq_dec_db.
 Hint Resolve exn_eq_dec : eq_dec_db.
 Hint Resolve eff_eq_dec : eq_dec_db.
-Hint Resolve variant_eq_dec : eq_dec_db.
-Hint Resolve record_eq_dec : eq_dec_db.
