shift-reset/core/record.v
@@ -5,3 +5,12 @@ Fixpoint record_lookup (tag : tag) (r : record) : option val :=
   | RecordNil => None
   | RecordCons tag' v r' => if tag_eqb tag tag' then Some v else record_lookup tag r'
   end.
+
+Fixpoint record_lookup_remove (tag : tag) (r : record) : option val * record :=
+  match r with
+  | RecordNil => (None, r)
+  | RecordCons tag' v r' =>
+      if tag_eqb tag tag'
+      then (Some v, r')
+      else let (o, r') := record_lookup_remove tag r' in (o, RecordCons tag' v r')
+  end.
