shift-reset/core/syntax_notation.v
@@ -1,4 +1,4 @@
-From shift_reset.core Require Import syntax tag.
+From shift_reset.core Require Import syntax.
 
 Declare Scope term_scope.
 Delimit Scope term_scope with term.
@@ -6,10 +6,9 @@ Bind Scope term_scope with term.
 Local Open Scope term_scope.
 
 Declare Custom Entry binder'.
-Declare Custom Entry pattern'.
+Declare Custom Entry variant_pattern.
+Declare Custom Entry record_pattern.
 Declare Custom Entry term.
-Declare Custom Entry term1.
-Declare Custom Entry term2.
 Declare Custom Entry ret_term.
 Declare Custom Entry exn_term.
 Declare Custom Entry eff_term.
@@ -19,26 +18,20 @@ Declare Custom Entry record_term.
 Notation "'_'" := BAny (in custom binder' at level 0) : term_scope.
 Notation "x" := x (in custom binder' at level 0, x constr at level 0) : term_scope.
 
-Notation "'_'" := PAny (in custom pattern' at level 0) : term_scope.
-Notation "( x )" := x (in custom pattern', x at level 99) : term_scope.
-Notation "x" := x (in custom pattern' at level 0, x constr at level 0) : term_scope.
+Notation "'_'" := PVariantAny (in custom variant_pattern at level 0) : term_scope.
+Notation "x" := x (in custom variant_pattern at level 0, x constr at level 0) : term_scope.
 
-Notation "' tag" :=
-  (PConstr tag nil) (in custom pattern' at level 10, tag constr at level 0) : term_scope.
-
-Notation "' tag x1 .. xn" :=
-  (PConstr tag (cons (x1 : binder) .. (cons (xn : binder) nil) ..))
-    (in custom pattern' at level 10,
+Notation "' ( tag x )" :=
+  (PVariantTag tag x)
+    (in custom variant_pattern at level 0,
         tag constr at level 0,
-        x1 custom binder' at level 0,
-        xn custom binder' at level 0) : term_scope.
+        x custom binder' at level 0) : term_scope.
 
-Notation "x1 'as' x2" :=
-  (PAlias x1 x2)
-    (in custom pattern' at level 15,
-        x1 custom pattern',
-        x2 constr at level 0,
-        left associativity) : term_scope.
+Notation "` tag x" :=
+  (PVariantTag tag x)
+    (in custom variant_pattern at level 0,
+        tag constr at level 0,
+        x custom binder' at level 0) : term_scope.
 
 Notation "<{ t }>" := t (t custom term at level 99) : term_scope.
 Notation "( t )" := t (in custom term, t at level 99) : term_scope.
@@ -46,55 +39,45 @@ Notation "{ t }" := t (in custom term, t constr) : term_scope.
 Notation "t" := t (in custom term at level 0, t constr at level 0) : term_scope.
 
 Notation "( 'fun' x => t )" :=
-  (T1 x t) (in custom term1 at level 69, x custom binder' at level 0, t custom term) : term_scope.
-
-Notation "( 'fun' x1 x2 => t )" :=
-  (T2 x1 x2 t)
-    (in custom term2 at level 69,
-        x1 custom binder' at level 0,
-        x2 custom binder' at level 0,
-        t custom term) : term_scope.
-
-Notation "( 'fun' x => t )" :=
   (TRetSome x t) (in custom ret_term at level 69, x custom binder' at level 0, t custom term) : term_scope.
 
-Notation "( 'fun' x => t )" :=
-  (TExnLast x t) (in custom exn_term at level 69, x custom pattern' at level 15, t custom term) : term_scope.
+Notation "( 'fun' p => t )" :=
+  (TExnLast p t) (in custom exn_term at level 69, p custom variant_pattern at level 0, t custom term) : term_scope.
 
-Notation "( 'fun' x => t1 ) ; t2" :=
-  (TExnCons x t1 t2)
+Notation "( 'fun' p => t1 ) ; t2" :=
+  (TExnCons p t1 t2)
     (in custom exn_term at level 69,
-        x custom pattern' at level 15,
+        p custom variant_pattern at level 0,
         t1 custom term,
         t2 custom exn_term,
         right associativity) : term_scope.
 
-Notation "( 'fun' x , k => t )" :=
-  (TEffLast x k t)
+Notation "( 'fun' p , k => t )" :=
+  (TEffLast p k t)
     (in custom eff_term at level 69,
-        x custom pattern' at level 15,
+        p custom variant_pattern at level 0,
         k custom binder' at level 0,
         t custom term) : term_scope.
 
-Notation "( 'fun' x , k => t1 ) ; t2" :=
-  (TEffCons x k t1 t2)
+Notation "( 'fun' p , k => t1 ) ; t2" :=
+  (TEffCons p k t1 t2)
     (in custom eff_term at level 69,
-        x custom pattern' at level 15,
+        p custom variant_pattern at level 0,
         k custom binder' at level 0,
         t1 custom term,
         t2 custom eff_term,
         right associativity) : term_scope.
 
-Notation "| x => t" :=
-  (TVariantCons x t TVariantNil)
+Notation "| p => t" :=
+  (TVariantCons p t TVariantNil)
     (in custom variant_term at level 69,
-        x custom pattern' at level 15,
+        p custom variant_pattern at level 0,
         t custom term) : term_scope.
 
-Notation "| x => t1 t2" :=
-  (TVariantCons x t1 t2)
+Notation "| p => t1 t2" :=
+  (TVariantCons p t1 t2)
     (in custom variant_term at level 69,
-        x custom pattern' at level 15,
+        p custom variant_pattern at level 0,
         t1 custom term,
         t2 custom variant_term,
         right associativity) : term_scope.
@@ -102,15 +85,15 @@ Notation "| x => t1 t2" :=
 Notation "t1 t2" :=
   (TApp t1 t2) (in custom term at level 17, t1 custom term, t2 custom term) : term_scope.
 
-Notation "'if' t1 'then' t2 'else' t3" :=
-  (TIf t1 t2 t3)
+Notation "'if' tv 'then' t1 'else' t2" :=
+  (TIf tv t1 t2)
     (in custom term at level 69,
+        tv custom term,
         t1 custom term,
-        t2 custom term,
-        t3 custom term) : term_scope.
+        t2 custom term) : term_scope.
 
 Notation "'let' x := t1 'in' t2" :=
-  (TLet t1 (T1 x t2))
+  (TLet x t1 t2)
     (in custom term at level 69,
         x custom binder' at level 0,
         t1 custom term,
@@ -125,7 +108,7 @@ Notation "t1 ; t2" :=
         right associativity) : term_scope.
 
 Notation "'let' f x1 .. xn := t1 'in' t2" :=
-  (TLet (TVFun (T1 x1 .. (TVFun (T1 xn t1)) ..)) (T1 f t2))
+  (TLet f (TVFun x1 .. (TVFun xn t1) ..) t2)
     (in custom term at level 69,
         f custom binder' at level 0,
         x1 custom binder' at level 0,
@@ -135,18 +118,18 @@ Notation "'let' f x1 .. xn := t1 'in' t2" :=
         right associativity) : term_scope.
 
 Notation "'let' 'fix' f x := t1 'in' t2" :=
-  (TLet (TVFix (T2 f x t1)) (T1 f t2))
+  (TLetFix f x t1 t2)
     (in custom term at level 69,
-        f custom binder' at level 0,
+        f constr at level 0,
         x custom binder' at level 0,
         t1 custom term,
         t2 custom term,
         right associativity) : term_scope.
 
 Notation "'let' 'fix' f x1 x2 .. xn := t1 'in' t2" :=
-  (TLet (TVFix (T2 f x1 (TVFun (T1 x2 .. (TVFun (T1 xn t1)) ..)))) (T1 f t2))
+  (TLetFix f x1 (TVFun x2 .. (TVFun xn t1) ..) t2)
     (in custom term at level 69,
-        f custom binder' at level 0,
+        f constr at level 0,
         x1 custom binder' at level 0,
         x2 custom binder' at level 0,
         xn custom binder' at level 0,
@@ -154,49 +137,37 @@ Notation "'let' 'fix' f x1 x2 .. xn := t1 'in' t2" :=
         t2 custom term,
         right associativity) : term_scope.
 
-Notation "'while' t1 'do' t2" :=
-  (TWhile t1 t2) (in custom term at level 69, t1 custom term, t2 custom term) : term_scope.
+Notation "'while' tv 'do' t" :=
+  (TWhile tv t) (in custom term at level 69, tv custom term, t custom term) : term_scope.
 
-Notation "'shift' t" :=
-  (TShift tag_empty t) (in custom term at level 69, t custom term1) : term_scope.
+Notation "'shift' ( 'fun' k => t )" :=
+  (TShift k t) (in custom term at level 69, k custom binder' at level 0, t custom term) : term_scope.
 
-Notation "'shift' 'at' tag t" :=
-  (TShift tag t) (in custom term at level 69, tag constr at level 0, t custom term1) : term_scope.
-
-Notation "'control' t" :=
-  (TControl tag_empty t) (in custom term at level 69, t custom term1) : term_scope.
-
-Notation "'control' 'at' tag t" :=
-  (TControl tag t) (in custom term at level 69, tag constr at level 0, t custom term1) : term_scope.
+Notation "'control' ( 'fun' k => t )" :=
+  (TControl k t) (in custom term at level 69, k custom binder' at level 0, t custom term) : term_scope.
 
 Notation "'reset' t" :=
-  (TReset tag_empty t) (in custom term at level 69, t custom term) : term_scope.
-
-Notation "'reset' 'at' tag t" :=
-  (TReset tag t) (in custom term at level 69, tag constr at level 0, t custom term) : term_scope.
+  (TReset t) (in custom term at level 69, t custom term) : term_scope.
 
 Notation "'prompt' t" :=
-  (TPrompt tag_empty t) (in custom term at level 69, t custom term) : term_scope.
-
-Notation "'prompt' 'at' tag t" :=
-  (TPrompt tag t) (in custom term at level 69, tag constr at level 0, t custom term) : term_scope.
+  (TPrompt t) (in custom term at level 69, t custom term) : term_scope.
 
 Notation "'fun' x1 .. xn => t" :=
-  (TVFun (T1 x1 .. (TVFun (T1 xn t)) ..))
+  (TVFun x1 .. (TVFun xn t) ..)
     (in custom term at level 69,
         x1 custom binder' at level 0,
         xn custom binder' at level 0,
         t custom term at level 99) : term_scope.
 
 Notation "'fix' f x := t" :=
-  (TVFix (T2 f x t))
+  (TVFix f x t)
     (in custom term at level 69,
         f custom binder' at level 0,
         x custom binder' at level 0,
         t custom term at level 99) : term_scope.
 
 Notation "'fix' f x1 x2 .. xn := t" :=
-  (TVFix (T2 f x1 (TVFun (T1 x2 .. (TVFun (T1 xn t)) ..))))
+  (TVFix f x1 (TVFun x2 .. (TVFun xn t) ..))
     (in custom term at level 69,
         f custom binder' at level 0,
         x1 custom binder' at level 0,
@@ -204,7 +175,7 @@ Notation "'fix' f x1 x2 .. xn := t" :=
         xn custom binder' at level 0,
         t custom term at level 99) : term_scope.
 
-Notation "()" := TVUnit (in custom term at level 0) : term_scope.
+Notation "()" := TVTt (in custom term at level 0) : term_scope.
 Notation "'true'" := TVTrue (in custom term at level 0) : term_scope.
 Notation "'false'" := TVFalse (in custom term at level 0) : term_scope.
 
@@ -274,22 +245,32 @@ Notation "t1 <- t2" :=
 Notation "t1 , t2" :=
   (TVPair t1 t2) (in custom term at level 65, t1 custom term, t2 custom term) : term_scope.
 
-Notation "'let' ( x1 , x2 ) := t1 'in' t2" :=
-  (TUnpair t1 (T2 x1 x2 t2))
+Notation "`( t1 , t2 , t3 , .. , tn )" :=
+  (TVTuple (TTupleCons t1 (TTupleCons t2 (TTupleCons t3 .. (TTupleCons tn TTupleNil) ..))))
+    (in custom term at level 65,
+        t1 custom term at level 23,
+        t2 custom term at level 23,
+        t3 custom term at level 23,
+        tn custom term at level 23) : term_scope.
+
+Notation "'let' ( x1 , x2 ) := tv 'in' t" :=
+  (TSplit x1 x2 tv t)
     (in custom term at level 69,
         x1 custom binder' at level 0,
         x2 custom binder' at level 0,
-        t1 custom term,
-        t2 custom term,
+        tv custom term,
+        t custom term,
         right associativity) : term_scope.
 
-Notation "'let' x1 , x2 := t1 'in' t2" :=
-  (TUnpair t1 (T2 x1 x2 t2))
+Notation "'let' ( x1 , x2 , x3 , .. , xn ) := tv 'in' t" :=
+  (TLetTuple (PTupleCons x1 (PTupleCons x2 (PTupleCons x3 .. (PTupleCons xn PTupleNil) ..))) tv t)
     (in custom term at level 69,
         x1 custom binder' at level 0,
         x2 custom binder' at level 0,
-        t1 custom term,
-        t2 custom term,
+        x3 custom binder' at level 0,
+        xn custom binder' at level 0,
+        tv custom term,
+        t custom term,
         right associativity) : term_scope.
 
 Notation "'Inl' t" :=
@@ -299,7 +280,7 @@ Notation "'Inr' t" :=
   (TVInr t) (in custom term at level 23, t custom term at level 0) : term_scope.
 
 Notation "'match' tv 'with' | 'Inl' x1 => t1 | 'Inr' x2 => t2 'end'" :=
-  (TCase tv (T1 x1 t1) (T1 x2 t2))
+  (TCase tv x1 t1 x2 t2)
     (in custom term at level 69,
         tv custom term,
         x1 custom binder' at level 0,
@@ -307,15 +288,11 @@ Notation "'match' tv 'with' | 'Inl' x1 => t1 | 'Inr' x2 => t2 'end'" :=
         t1 custom term,
         t2 custom term) : term_scope.
 
-Notation "'exception' tag" :=
-  (TVExn tag nil) (in custom term at level 23, tag constr at level 0) : term_scope.
-
-Notation "'exception' tag t1 .. tn" :=
-  (TVExn tag (cons (t1 : val_term) .. (cons (tn : val_term) nil) ..))
+Notation "'exception' tag t" :=
+  (TVExn tag t)
     (in custom term at level 23,
         tag constr at level 0,
-        t1 custom term at level 0,
-        tn custom term at level 0) : term_scope.
+        t custom term at level 0) : term_scope.
 
 Notation "'raise' t" :=
   (TRaise t) (in custom term at level 23, t custom term at level 0) : term_scope.
@@ -323,15 +300,11 @@ Notation "'raise' t" :=
 Notation "'try' t1 ;; t2" :=
   (TTry t1 t2) (in custom term at level 69, t1 custom term, t2 custom exn_term) : term_scope.
 
-Notation "'effect' tag" :=
-  (TVEff tag nil) (in custom term at level 23, tag constr at level 0) : term_scope.
-
-Notation "'effect' tag t1 .. tn" :=
-  (TVEff tag (cons (t1 : val_term) .. (cons (tn : val_term) nil) ..))
+Notation "'effect' tag t" :=
+  (TVEff tag t)
     (in custom term at level 23,
         tag constr at level 0,
-        t1 custom term at level 0,
-        tn custom term at level 0) : term_scope.
+        t custom term at level 0) : term_scope.
 
 Notation "'perform' t" :=
   (TPerform t) (in custom term at level 23, t custom term at level 0) : term_scope.
@@ -362,18 +335,14 @@ Notation "'shallow' 'handle' t1 ;;; t2" :=
         t1 custom term,
         t2 custom eff_term) : term_scope.
 
-Notation "` tag" :=
-  (TVVariant tag nil) (in custom term at level 23, tag constr at level 0) : term_scope.
-
-Notation "` tag t1 .. tn" :=
-  (TVVariant tag (cons (t1 : val_term) .. (cons (tn : val_term) nil) ..))
+Notation "` tag t" :=
+  (TVVariant tag t)
     (in custom term at level 23,
         tag constr at level 0,
-        t1 custom term at level 0,
-        tn custom term at level 0) : term_scope.
+        t custom term at level 0) : term_scope.
 
-Notation "'match' t1 'with' t2 'end'" :=
-  (TMatch t1 t2) (in custom term at level 69, t1 custom term, t2 custom variant_term) : term_scope.
+Notation "'match' tv 'with' t 'end'" :=
+  (TMatchVariant tv t) (in custom term at level 69, tv custom term, t custom variant_term) : term_scope.
 
 Notation "`{ tag := t1 t2" :=
   (TVRecord (TRecordCons tag t1 t2))
