shift-reset/interpreter/ierror.v
@@ -1,18 +1,16 @@
 From Stdlib Require Import String.
-From shift_reset.core Require Import syntax tag var.
 
 Local Unset Elimination Schemes.
 
 Inductive ierror : Type :=
 | Failure : string -> ierror
 | Type_error : string -> ierror
-| Name_error : var -> ierror
+| Name_error : string -> ierror
 | Memory_error : string -> ierror
 | Assert_failure : string -> ierror
 | Match_failure : string -> ierror
-| Projection_failure : string -> ierror
-| Undelimited_shift : tag -> ierror
-| Undelimited_control : tag -> ierror
-| Unhandled_exception : exn -> ierror
-| Unhandled_effect : eff -> ierror
+| Undelimited_shift : string -> ierror
+| Undelimited_control : string -> ierror
+| Unhandled_exception : string -> ierror
+| Unhandled_effect : string -> ierror
 | Out_of_fuel : ierror.
